txn-data-consistency/Prot_2PC_2PL.thy
@@ -8,117 +8,120 @@ subsection \<open>2PC Event system\<close>
 
 subsubsection \<open>State\<close>
 
-datatype status_rm = working | prepared | okay | notokay | committed | aborted
+datatype status_rm = working | prepared | read_lock | write_lock | notokay | committed | aborted
 datatype status_tm = tm_init | tm_prepared | tm_committed | tm_aborted
 
 record tm_state =
   tm_status :: status_tm
-  tm_tid :: txid0
-  tm_view :: view
-
-typedecl rmid
-consts loc :: "key \<Rightarrow> rmid"
+  tm_sn :: nat
+  (*tm_view :: view*)
 
 record 'v rm_state =
-  rm_db :: "'v kv_store"
-  rm_fingerpr :: "'v fingerpr"
-  rm_status :: status_rm
-  rm_tid :: txid0
-
-type_synonym 'v rms_state = "rmid \<Rightarrow> 'v rm_state"
+  rm_db :: "'v version list"
+  rm_fingerpr :: "txid0 \<Rightarrow> 'v key_fp"
+  rm_status :: "txid0 \<Rightarrow> status_rm"
 
 record 'v global_state =
-  tm :: tm_state
-  rms :: "'v rms_state"
+  tm :: "cl_id \<Rightarrow> tm_state"
+  rms :: "key \<Rightarrow> 'v rm_state"
 
 
 subsubsection \<open>Events\<close>
 
-datatype 'v ev = Write2 rmid key 'v | Read2 rmid key 'v |
-                 Prepare rmid | OK rmid | NOK rmid | Commit rmid | Abort rmid | Ready rmid |
-                 User_Commit | TM_Commit | TM_Abort | TM_ReadyC | TM_ReadyA | TM_Skip
+datatype 'v rm_ev = Write2 txid0 'v | Read2 txid0 'v | Prepare txid0 | RLock txid0 | WLock txid0 |
+                 NOK txid0 | Commit txid0 | Abort txid0 | Ready txid0
+datatype tm_ev = User_Commit | TM_Commit | TM_Abort | TM_ReadyC | TM_ReadyA | TM_Skip
+datatype 'v ev = RM_ev key "'v rm_ev" | TM_ev cl_id tm_ev
+
+definition other_instances_unchanged where
+  "other_instances_unchanged t k rmss rmss' \<equiv> (\<forall>t'. t' \<noteq> t \<longrightarrow>
+     rm_fingerpr (rmss' k) t' = rm_fingerpr (rmss k) t' \<and>
+     rm_status (rmss' k) t' = rm_status (rmss k) t')"
 
 definition other_rms_unchanged where
-  "other_rms_unchanged rm rmss rmss' \<equiv> (\<forall>rm'. rm' \<noteq> rm \<longrightarrow> rmss' rm' = rmss rm')"
+  "other_rms_unchanged k rmss rmss' \<equiv> (\<forall>k'. k' \<noteq> k \<longrightarrow> rmss' k' = rmss k')"
 
 abbreviation tm_other_rms_unchanged where
-  "tm_other_rms_unchanged rm s s' \<equiv> tm s' = tm s \<and> other_rms_unchanged rm (rms s) (rms s')"
-
-abbreviation tid_match where
-  "tid_match s rm \<equiv> rm_tid (rms s rm) = tm_tid (tm s)"
+  "tm_other_rms_unchanged t k s s' \<equiv> tm s' = tm s \<and>
+    other_rms_unchanged k (rms s) (rms s') \<and> other_instances_unchanged t k (rms s) (rms s')"
 
 abbreviation rm_status_trans where
-  "rm_status_trans s rm s' from_stat to_stat \<equiv>
-      rm_status (rms s rm) = from_stat
-    \<and> rm_db (rms s' rm) = rm_db (rms s rm)
-    \<and> rm_fingerpr (rms s' rm) = rm_fingerpr (rms s rm)
-    \<and> rm_status (rms s' rm) = to_stat
-    \<and> rm_tid (rms s' rm) = rm_tid (rms s rm)
-    \<and> tm_other_rms_unchanged rm s s'"
+  "rm_status_trans s k s' t from_stat to_stat \<equiv>
+      rm_status (rms s k) t = from_stat
+    \<and> rm_db (rms s' k) = rm_db (rms s k)
+    \<and> rm_fingerpr (rms s' k) = rm_fingerpr (rms s k)
+    \<and> rm_status (rms s' k) t = to_stat
+    \<and> tm_other_rms_unchanged t k s s'"
 
 fun tid_inc :: "txid0 \<Rightarrow> txid0" where
   "tid_inc (Tn_cl sn cl) = Tn_cl (Suc sn) cl"
 
 definition write2 where
-  "write2 s rm k v s' \<equiv> loc k = rm
-                        \<and> rm_status (rms s rm) = working
-                        \<and> tid_match s rm
-                        \<and> rm_fingerpr (rms s' rm) = update_fp (rm_fingerpr (rms s rm)) (Write k v)
-                        \<and> rm_status (rms s' rm) = working
-                        \<and> rm_db (rms s' rm) = rm_db (rms s rm)
-                        \<and> rm_tid (rms s' rm) = rm_tid (rms s rm)
-                        \<and> tm_other_rms_unchanged rm s s'"
+  "write2 s k v s' cl \<equiv> let t = (Tn_cl (tm_sn (tm s cl)) cl) in 
+                          rm_status (rms s k) t = working
+                        \<and> rm_fingerpr (rms s' k) t = update_key_fp (rm_fingerpr (rms s k) t) W v
+                        \<and> rm_status (rms s' k) t = working
+                        \<and> rm_db (rms s' k) = rm_db (rms s k)
+                        \<and> tm_other_rms_unchanged t k s s'"
 
 definition read2 where
-  "read2 s rm k v s' \<equiv> loc k = rm 
-                        \<and> rm_status (rms s rm) = working
-                        \<and> tid_match s rm
-                        \<and> rm_fingerpr (rms s' rm) = update_fp (rm_fingerpr (rms s rm)) (Read k v)
-                        \<comment> \<open>\<and> ov = (rm_main_db (rms s rm) ++ rm_shadow_db (rms s rm)) k\<close>
-                        \<and> rm_status (rms s' rm) = working
-                        \<and> rm_db (rms s' rm) = rm_db (rms s rm)
-                        \<and> rm_tid (rms s' rm) = rm_tid (rms s rm)
-                        \<and> tm_other_rms_unchanged rm s s'"
+  "read2 s v k s' cl  \<equiv> let t = (Tn_cl (tm_sn (tm s cl)) cl) in
+                          rm_status (rms s k) t = working
+                        \<and> rm_fingerpr (rms s' k) t = update_key_fp (rm_fingerpr (rms s k) t) R v
+                        \<and> rm_status (rms s' k) t = working
+                        \<and> rm_db (rms s' k) = rm_db (rms s k)
+                        \<and> tm_other_rms_unchanged t k s s'"
 
 definition prepare where
-  "prepare s rm s' \<equiv> tm_status (tm s) = tm_prepared
-                      \<and> rm_status_trans s rm s' working prepared"
+  "prepare s k s' cl \<equiv> tm_status (tm s cl) = tm_prepared
+                      \<and> rm_status_trans s k s' (Tn_cl (tm_sn (tm s cl)) cl) working prepared"
 
-definition ok where \<comment>\<open>Lock acquired\<close>
-  "ok s rm s' \<equiv> tm_status (tm s) = tm_prepared
-                \<and> rm_status_trans s rm s' prepared okay"
+definition acquire_rd_lock where \<comment>\<open>Read Lock acquired\<close>
+  "acquire_rd_lock s k s' cl \<equiv> let t = (Tn_cl (tm_sn (tm s cl)) cl) in 
+                   tm_status (tm s cl) = tm_prepared
+                  \<and> rm_fingerpr (rms s k) t W = None
+                  \<and> (rm_fingerpr (rms s k) t R = None \<or>
+                      (rm_fingerpr (rms s k) t R \<noteq> None \<and>
+                      (\<forall>t'. rm_status (rms s k) t' \<in> {working, prepared, read_lock, notokay})))
+                  \<and> rm_status_trans s k s' t prepared read_lock"
+
+definition acquire_rd_lock where \<comment>\<open>Write Lock acquired\<close>
+  "acquire_rd_lock s k s' cl \<equiv> let t = (Tn_cl (tm_sn (tm s cl)) cl) in 
+                   tm_status (tm s cl) = tm_prepared
+                  \<and> rm_fingerpr (rms s k) t W = None
+                  \<and> rm_status_trans s k s' t prepared read_lock"
 
 definition nok where \<comment>\<open>Lock not available\<close>
   "nok s rm s' \<equiv> tm_status (tm s) = tm_prepared
                 \<and> rm_status_trans s rm s' prepared notokay"
 
 definition commit where
-  "commit s rm s' \<equiv> rm_status (rms s rm) = okay
+  "commit s rm s' \<equiv> rm_status (rms s k) = okay
                     \<and> tm_status (tm s) = tm_committed
-                    \<and> rm_db (rms s' rm) =  update_kv (rm_tid (rms s rm)) (rm_fingerpr (rms s rm))
-                                                     (tm_view (tm s)) (rm_db (rms s rm)) \<comment>\<open>?\<close>
-                    \<and> rm_fingerpr (rms s' rm) = Map.empty
-                    \<and> rm_status (rms s' rm) = committed
-                    \<and> rm_tid (rms s' rm) = rm_tid (rms s rm)
+                    \<and> rm_db (rms s' k) =  update_kv (rm_tid (rms s k)) (rm_fingerpr (rms s k))
+                                                     (tm_view (tm s)) (rm_db (rms s k)) \<comment>\<open>?\<close>
+                    \<and> rm_fingerpr (rms s' k) = Map.empty
+                    \<and> rm_status (rms s' k) = committed
+                    \<and> rm_tid (rms s' k) = rm_tid (rms s k)
                     \<and> tm_other_rms_unchanged rm s s'"
 
 definition abort where \<comment>\<open>Lock released (if starting from okay)\<close>
-  "abort s rm s' \<equiv> (rm_status (rms s rm) = okay \<or>
-                    rm_status (rms s rm) = notokay)
+  "abort s rm s' \<equiv> (rm_status (rms s k) = okay \<or>
+                    rm_status (rms s k) = notokay)
                     \<and> tm_status (tm s) = tm_aborted
-                    \<and> rm_db (rms s' rm) = rm_db (rms s rm)
-                    \<and> rm_fingerpr (rms s' rm) = Map.empty
-                    \<and> rm_status (rms s' rm) = aborted
-                    \<and> rm_tid (rms s' rm) = rm_tid (rms s rm)
+                    \<and> rm_db (rms s' k) = rm_db (rms s k)
+                    \<and> rm_fingerpr (rms s' k) = Map.empty
+                    \<and> rm_status (rms s' k) = aborted
+                    \<and> rm_tid (rms s' k) = rm_tid (rms s k)
                     \<and> tm_other_rms_unchanged rm s s'"
 
 definition ready where \<comment>\<open>Lock released (if starting from committed)\<close>
-  "ready s rm s' \<equiv> ((rm_status (rms s rm) = committed \<and> tm_status (tm s) = tm_committed)
-                      \<or> (rm_status (rms s rm) = aborted \<and> tm_status (tm s) = tm_aborted))
-                   \<and> rm_status (rms s' rm) = working
-                   \<and> rm_tid (rms s' rm) = tid_inc (rm_tid (rms s rm))
-                   \<and> rm_db (rms s' rm) = rm_db (rms s rm)
-                   \<and> rm_fingerpr (rms s' rm) = rm_fingerpr (rms s rm)
+  "ready s rm s' \<equiv> ((rm_status (rms s k) = committed \<and> tm_status (tm s) = tm_committed)
+                      \<or> (rm_status (rms s k) = aborted \<and> tm_status (tm s) = tm_aborted))
+                   \<and> rm_status (rms s' k) = working
+                   \<and> rm_tid (rms s' k) = tid_inc (rm_tid (rms s k))
+                   \<and> rm_db (rms s' k) = rm_db (rms s k)
+                   \<and> rm_fingerpr (rms s' k) = rm_fingerpr (rms s k)
                    \<and> tm_other_rms_unchanged rm s s'"
 
 definition user_commit where
@@ -130,7 +133,7 @@ definition user_commit where
 
 definition tm_commit where
   "tm_commit s s' \<equiv> tm_status (tm s) = tm_prepared
-                    \<and> (\<forall>rm. rm_status (rms s rm) = okay)
+                    \<and> (\<forall>rm. rm_status (rms s k) = okay)
                     \<and> tm_status (tm s') = tm_committed
                     \<and> tm_tid (tm s') = tm_tid (tm s)
                     \<and> tm_view (tm s') = tm_view (tm s)
@@ -138,8 +141,8 @@ definition tm_commit where
 
 definition tm_abort where
   "tm_abort s s' \<equiv> (tm_status (tm s) = tm_prepared
-                     \<and> (\<exists>rm. rm_status (rms s rm) = notokay)
-                     \<and> (\<forall>rm. rm_status (rms s rm) = okay \<or> rm_status (rms s rm) = notokay))
+                     \<and> (\<exists>rm. rm_status (rms s k) = notokay)
+                     \<and> (\<forall>rm. rm_status (rms s k) = okay \<or> rm_status (rms s k) = notokay))
                     \<and> tm_status (tm s') = tm_aborted
                     \<and> tm_tid (tm s') = tm_tid (tm s)
                     \<and> tm_view (tm s') = tm_view (tm s)
@@ -147,7 +150,7 @@ definition tm_abort where
 
 definition tm_ready_c where
   "tm_ready_c s s' \<equiv> tm_status (tm s) = tm_committed
-                    \<and> (\<forall>rm. rm_status (rms s rm) = working \<and> rm_tid (rms s rm) = tid_inc (tm_tid (tm s)))
+                    \<and> (\<forall>rm. rm_status (rms s k) = working \<and> rm_tid (rms s k) = tid_inc (tm_tid (tm s)))
                     \<and> tm_status (tm s') = tm_init
                     \<and> tm_tid (tm s') = tid_inc (tm_tid (tm s))
                     \<and> tm_view (tm s') = tm_view (tm s) \<comment>\<open>Should see its own transaction?\<close>
@@ -155,7 +158,7 @@ definition tm_ready_c where
 
 definition tm_ready_a where
   "tm_ready_a s s' \<equiv> tm_status (tm s) = tm_aborted
-                    \<and> (\<forall>rm. rm_status (rms s rm) = working \<and> rm_tid (rms s rm) = tid_inc (tm_tid (tm s)))
+                    \<and> (\<forall>rm. rm_status (rms s k) = working \<and> rm_tid (rms s k) = tid_inc (tm_tid (tm s)))
                     \<and> tm_status (tm s') = tm_init
                     \<and> tm_tid (tm s') = tid_inc (tm_tid (tm s))
                     \<and> tm_view (tm s') = tm_view (tm s) \<comment>\<open>Should see its own transaction?\<close>
@@ -173,12 +176,12 @@ definition gs_init :: "'v global_state" where
 fun gs_trans :: "'v global_state \<Rightarrow> 'v ev \<Rightarrow> 'v global_state \<Rightarrow> bool" where
   "gs_trans s (Write2 rm k v) s' \<longleftrightarrow> write2 s rm k v s'" |
   "gs_trans s (Read2 rm k ov) s' \<longleftrightarrow> read2 s rm k ov s'" |
-  "gs_trans s (Prepare rm)    s' \<longleftrightarrow> prepare s rm s'" |
-  "gs_trans s (OK rm)         s' \<longleftrightarrow> ok s rm s'" |
-  "gs_trans s (NOK rm)        s' \<longleftrightarrow> nok s rm s'" |
-  "gs_trans s (Commit rm)     s' \<longleftrightarrow> commit s rm s'" |
-  "gs_trans s (Abort rm)      s' \<longleftrightarrow> abort s rm s'" |
-  "gs_trans s (Ready rm)      s' \<longleftrightarrow> ready s rm s'" |
+  "gs_trans s (Prepare k)    s' \<longleftrightarrow> prepare s rm s'" |
+  "gs_trans s (OK k)         s' \<longleftrightarrow> ok s rm s'" |
+  "gs_trans s (NOK k)        s' \<longleftrightarrow> nok s rm s'" |
+  "gs_trans s (Commit k)     s' \<longleftrightarrow> commit s rm s'" |
+  "gs_trans s (Abort k)      s' \<longleftrightarrow> abort s rm s'" |
+  "gs_trans s (Ready k)      s' \<longleftrightarrow> ready s rm s'" |
   "gs_trans s User_Commit     s' \<longleftrightarrow> user_commit s s'" |
   "gs_trans s TM_Commit       s' \<longleftrightarrow> tm_commit s s'" |
   "gs_trans s TM_Abort        s' \<longleftrightarrow> tm_abort s s'" |
@@ -192,7 +195,7 @@ definition tps :: "('v ev, 'v global_state) ES" where
     trans = gs_trans
   \<rparr>"
 
-lemmas tps_trans_defs = prepare_def ok_def nok_def (*commit_def*) abort_def ready_def
+lemmas tps_trans_defs = prepare_def ok_def nok_def commit_def abort_def ready_def
                         user_commit_def tm_commit_def tm_abort_def tm_ready_c_def tm_ready_a_def
 
 lemmas tps_defs = tps_def gs_init_def
